Lemmas/String/Instances.lean
@@ -4,7 +4,6 @@ import Std.Tactic.Do
 import Std.Tactic.Do.Syntax
 
 import Lemmas.Lemmas
-import Lemmas.String.Basic
 
 open Lean Lean.Syntax Parser Parser.Char
 
@@ -13,6 +12,18 @@ open Std.Do
 set_option mvcgen.warning false
 
 namespace Parser.String.Slice
+
+/- see https://github.com/fgdorais/lean4-parser/pull/99, remove when PR#99 is merged
+ -/
+instance : Parser.Stream.Remaining String.Slice where
+  remaining s := s.utf8ByteSize
+
+instance : Parser.Stream.ValidPosition String.Slice where
+  valid _ := True
+  validOfRemaining it h := by simp
+
+instance : Parser.Stream.AllValid String.Slice where
+  valid := by simp [Stream.ValidPosition.valid]
 
 @[simp] private def respectsPosition (it rem : String.Slice) :=
   it.str = rem.str ∧ it.endExclusive.offset = rem.endExclusive.offset
@@ -30,77 +41,67 @@ private theorem slice!PosEq (s : String) (p₁ p₂ : s.Pos) (h : p₁.offset �
   rw [← @String.Slice.slice_eq_slice! s p₁.toSlice p₂.toSlice h]
   simp
 
-private theorem getPositionOkEq (it : String.Slice)
-  (h : (getPosition : (SimpleParser String.Slice Char) _) it = Result.ok s a)
-    : it = s ∧ it.startInclusive.offset = a := by
-  have hg := getPositionSpec it (by simp)
-  simp [wp, Id.run, Stream.getPosition] at hg
-  and_intros <;> grind
-
 private theorem setPositionPrecondition (it : String.Slice) (pos : Stream.Position String.Slice)
   : pos.IsValid it.str ∧ pos ≤ it.endExclusive.offset
-    → ∃ r, (setPosition pos : (SimpleParser String.Slice Char) Unit) it = r
-      ∧ (∃ rem, r = Result.ok rem () ∧ pos = rem.startInclusive.offset
-                        ∧ respectsPosition it rem) := by
-  dsimp [setPosition, Stream.setPosition, getStream, setStream, pure,
-    Applicative.toPure, Monad.toApplicative, bind]
-  intro h
-  simp_all
-  have := slice!PosEq it.str ⟨pos, h.left⟩ ⟨it.endExclusive.offset, it.endExclusive.isValid⟩
+    → ∃ rem, Stream.setPosition it pos = rem
+              ∧ pos = Parser.Stream.getPosition rem
+              ∧ respectsPosition it rem := by
+  simp [Stream.setPosition, Stream.getPosition]
+  intro h1 h2
+  have := slice!PosEq it.str ⟨pos, by grind⟩ ⟨it.endExclusive.offset, it.endExclusive.isValid⟩
             (by simp_all)
-  grind
-
-private theorem setPositionEq (it : String.Slice) (pos)
-  (h : (setPosition pos : (SimpleParser String.Slice Char) Unit) it = Result.ok s ())
-  (hv : String.Pos.Raw.IsValid it.str pos) (hl2 : pos ≤ it.endExclusive.offset)
-    : s.startInclusive.offset = pos ∧ respectsPosition it s := by
-  rw [String.Pos.Raw.ext_iff]
-  have := setPositionPrecondition it pos (by solve_by_elim)
-  grind
+  generalize hg : (if h : String.Pos.Raw.IsValid it.str pos
+      then it.str.slice! { offset := pos, isValid := by grind } it.endExclusive
+      else default) = s
+  and_intros
+  · split at hg
+    · rw [← hg, this.left]
+    · simp_all
+  · simp_all
+  · split at hg
+    · rw [← hg, this.right.left]
+    · simp_all
 
 /-- no input is consumed if the position is reset after applying a respectful parser -/
-private theorem setPositionOfGetPositionEqIfRespectsPosition (s1 s2 s3 s4 : String.Slice)
-  (h1 : (getPosition : (SimpleParser String.Slice Char) _) s1 = Result.ok s2 p)
-  (h2 : respectsPosition s2 s3)
-  (h3 : (setPosition p : (SimpleParser String.Slice Char) Unit) s3 = Result.ok s4 ())
-    : s1 = s4 := by
-  simp_all
-  have := getPositionOkEq s1 h1
-  have := setPositionEq s3 p h3 (by grind [s1.startInclusive.isValid]) (by
-    have : p ≤ s2.endExclusive.offset := by
-      rw [this.left] at this
-      rw [← this.right]
-      exact s2.startInclusive_le_endExclusive
-    simp_all)
-  have : s1 = s2 := by grind
-  have : s1.startInclusive.offset = s4.startInclusive.offset := by grind
-  have : s1.endExclusive.offset = s4.endExclusive.offset := by simp_all; grind
-  expose_names
-  exact @String.Slice.ext s1 s4 (by simp_all)
-    (by
-      dsimp [String.Pos.cast]; simp_all;
-      exact String.Pos.ext_iff.mpr (id (Eq.symm this_2.left)))
-    (by dsimp [String.Pos.cast]; simp_all)
+private theorem setPositionOfGetPositionEqIfRespectsPosition (s1 s2 : String.Slice) (p)
+  (h1 : Stream.getPosition s1 = p) (h2 : respectsPosition s1 s2)
+    : Stream.setPosition s2 p = s1 := by
+  simp [Stream.getPosition] at h1
+  simp [respectsPosition] at h2
+  simp [Stream.setPosition]
+  have : String.Pos.Raw.IsValid s2.str p := by
+    rw [← h1, ← h2.left]
+    exact s1.startInclusive.isValid
+  split
+  · have := slice!PosEq s2.str ⟨p, by grind⟩ ⟨s2.endExclusive.offset, s2.endExclusive.isValid⟩
+            (by simp; rw [← h2.right, ← h1]; exact s1.startInclusive_le_endExclusive)
+    have := @String.Slice.ext
+      (s2.str.slice! { offset := p, isValid := by grind } s2.endExclusive) s1
+      (by simp_all)
+      (by simp [String.Pos.cast, String.Pos.ext_iff]; simp_all)
+      (by simp [String.Pos.cast, String.Pos.ext_iff]; simp_all)
+    simp_all
+  · simp_all
 
 instance : Stream.RespectsPosition String.Slice Char where
   respectsPosition := respectsPosition
-  setPositionOfGetPositionEq s1 s2 s3 s4 :=
-    fun h => setPositionOfGetPositionEqIfRespectsPosition s1 s2 s3 s4
-  respectsPositionEq (it) := by simp [respectsPosition]
+  setPositionOfGetPositionEq s1 s2 p :=
+    fun h => setPositionOfGetPositionEqIfRespectsPosition s1 s2 p
+  isEquivalence := Equivalence.mk (by simp) (by simp; grind) (by simp; grind)
 
 instance : Stream.SetPositionPrecondition String.Slice Char where
   cond it pos := pos.IsValid it.str ∧ pos ≤ it.endExclusive.offset
   validResult it pos := setPositionPrecondition it pos
-  ofGetPosition (s1 s2 s3 : String.Slice) (p : Stream.Position String.Slice) := by
+  ofGetPosition (s1 s2 : String.Slice) (p : Stream.Position String.Slice) := by
     intro _ h1 h2
-    have := getPositionOkEq s1 h1
+    simp [Stream.getPosition] at h1
     simp [Stream.RespectsPosition.respectsPosition] at h2
     and_intros
-    · grind [s1.startInclusive.isValid]
+    · rw [← h1, ← h2.left]
+      exact s1.startInclusive.isValid
     · have : p ≤ s2.endExclusive.offset := by
-        rw [this.left] at this
-        rw [← this.right]
-        exact s2.startInclusive_le_endExclusive
+        rw [← h1, ← h2.right]
+        exact s1.startInclusive_le_endExclusive
       simp_all
 
 @[simp, grind .] private theorem eqOfRemaining (it : String.Slice)
@@ -163,7 +164,7 @@ private theorem next?SomeOfLt (it : String.Slice)
     split at heq
     · grind
     · have := String.Pos.Raw.lt_iff.mpr (sliceOfNextLt it (by grind))
-      simp_all
+      simp_all [Stream.decrementsRemaining]
       have := Char.utf8Size_pos a
       grind
 
