Lemmas/Substring/Instances.lean
@@ -4,7 +4,6 @@ import Std.Tactic.Do
 import Std.Tactic.Do.Syntax
 
 import Lemmas.Lemmas
-import Lemmas.Substring.Basic
 
 open Lean Lean.Syntax Parser Parser.Char
 
@@ -13,6 +12,18 @@ open Std.Do
 set_option mvcgen.warning false
 
 namespace Parser.Substring.Raw
+
+/- see https://github.com/fgdorais/lean4-parser/pull/99, remove when PR#99 is merged
+ -/
+instance : Parser.Stream.Remaining Substring.Raw where
+  remaining s := s.bsize
+
+instance : Parser.Stream.ValidPosition Substring.Raw where
+  valid s := s.startPos ≤ s.stopPos
+  validOfRemaining it h := by
+    simp [Stream.Remaining.remaining, Substring.Raw.bsize] at h
+    rw [String.Pos.Raw.le_iff]
+    grind
 
 @[simp] private def respectsPosition (it rem : Substring.Raw) :=
   it.str = rem.str ∧ it.stopPos = rem.stopPos
@@ -26,61 +37,53 @@ private theorem getPositionOkEq (it : Substring.Raw)
 
 private theorem setPositionPrecondition (it : Substring.Raw) (pos :String.Pos.Raw)
   : pos ≤ it.stopPos
-    → ∃ r, (setPosition pos : (SimpleParser Substring.Raw Char) Unit) it = r
-      ∧ (∃ rem, r = Result.ok rem () ∧ pos = rem.startPos ∧ respectsPosition it rem) := by
+    → ∃ rem, Stream.setPosition it pos = rem
+                          ∧ pos = Parser.Stream.getPosition rem
+                          ∧ respectsPosition it rem := by
   dsimp [setPosition, Stream.setPosition, getStream, setStream, pure,
     Applicative.toPure, Monad.toApplicative, bind]
   intro h
   simp_all
   grind
 
-private theorem setPositionEq (it : Substring.Raw) (pos)
-  (h : (setPosition pos : (SimpleParser Substring.Raw Char) Unit) it = Result.ok s ())
-  (h : pos ≤ it.stopPos)
-    : s.startPos = pos ∧ respectsPosition it s := by
-  rw [String.Pos.Raw.ext_iff]
-  have := setPositionPrecondition it pos (by solve_by_elim)
-  grind
-
 /-- no input is consumed if the position is reset after applying a respectful parser -/
-private theorem setPositionOfGetPositionEqIfRespectsPosition (s1 s2 s3 s4 : Substring.Raw )
+private theorem setPositionOfGetPositionEqIfRespectsPosition (s1 s2 : Substring.Raw ) (p)
   (h0 : Stream.ValidPosition.valid s1)
-  (h1 : (getPosition : (SimpleParser Substring.Raw  Char) _) s1 = Result.ok s2 p)
-  (h2 : respectsPosition s2 s3)
-  (h3 : (setPosition p : (SimpleParser Substring.Raw  Char) Unit) s3 = Result.ok s4 ())
-    : s1 = s4 := by
+  (h1 : Stream.getPosition s1 = p) (h2 : respectsPosition s1 s2)
+    : Stream.setPosition s2 p = s1 := by
+  simp [Stream.ValidPosition.valid] at h0
+  simp [Stream.getPosition] at h1
+  simp [respectsPosition] at h2
+  simp [Stream.setPosition]
   simp_all
-  have := getPositionOkEq s1 h1
-  have := setPositionEq s3 p h3 (by simp [Stream.ValidPosition.valid] at h0; grind)
-  have : s1 = s2 := by grind
-  have : s1.str = s4.str := by simp_all
-  have : s1.startPos = s4.startPos := by grind
-  have : s1.stopPos = s4.stopPos := by simp_all
+  generalize h : ({ str := s2.str, startPos := p, stopPos := s2.stopPos } : Substring.Raw) = rem
+  have : s1.str = rem.str := by grind
+  have : s1.startPos = rem.startPos := by grind
+  have : s1.stopPos = rem.stopPos := by grind
   cases s1
-  cases s4
+  cases rem
   grind
 
 instance : Stream.RespectsPosition Substring.Raw Char where
   respectsPosition := respectsPosition
   setPositionOfGetPositionEq := setPositionOfGetPositionEqIfRespectsPosition
-  respectsPositionEq (it) := by simp [respectsPosition]
+  isEquivalence := Equivalence.mk (by simp) (by simp; grind) (by simp; grind)
 
 instance : Stream.SetPositionPrecondition Substring.Raw Char where
   cond it pos := pos ≤ it.stopPos
   validResult it pos := setPositionPrecondition it pos
-  ofGetPosition (s1 s2 s3 : Substring.Raw) (p : Stream.Position Substring.Raw) := by
-    intro h0 h1 h2
-    have := getPositionOkEq s1 h1
-    simp [Stream.RespectsPosition.respectsPosition] at h2
-    simp [Stream.ValidPosition.valid] at h0
-    grind
+  ofGetPosition (s1 s2 : Substring.Raw) (p : Stream.Position Substring.Raw) := by
+    simp [Stream.ValidPosition.valid, Stream.getPosition,
+          Stream.RespectsPosition.respectsPosition]
+    intros
+    simp_all
 
 private theorem next?SomeOfLt (it : Substring.Raw)
   (h : 0 < Stream.Remaining.remaining it)
     : ∃ rem c, Std.Stream.next? it = some (c, rem) ∧ Stream.decrementsRemaining it rem
                                   ∧ respectsPosition it rem := by
   simp [Stream.Remaining.remaining, Substring.Raw.bsize] at h
-  simp [Std.Stream.next?, Stream.Remaining.remaining, String.Pos.Raw.next]
+  simp [Std.Stream.next?, String.Pos.Raw.next]
   exact ⟨{str := it.str,
           startPos := it.startPos + String.Pos.Raw.get it.str it.startPos,
           stopPos := it.stopPos }, by
@@ -88,7 +91,7 @@ private theorem next?SomeOfLt (it : Substring.Raw)
     · rw [String.Pos.Raw.lt_iff]
       grind
     · rfl
-    · simp [HAdd.hAdd, Substring.Raw.bsize]
+    · simp [HAdd.hAdd]
       have h1 : 0 < (String.Pos.Raw.get it.str it.startPos).utf8Size :=
         Char.utf8Size_pos (String.Pos.Raw.get it.str it.startPos)
       exact Nat.sub_lt_sub_left (by grind) (by grind)
